Introduce GhostArray type and do some refactoring of creating calls

test-engine/src/main/java/com/aws/jverify/testengine/JVerifyTestEngine.java
@@ -195,15 +195,16 @@ public class JVerifyTestEngine extends HierarchicalTestEngine<EngineExecutionCon
             }
         }
 
+        assertThat("exit code",
+                verificationResults.getExitCode(),
+                is(annotation.exitCode()));
+        
         var expectedAnnotations = ranges.stream().sorted().toList();
         assertThat("diagnostics", diagnosticsAsAnnotations, equalTo(expectedAnnotations));
 
         Integer expectedDafnyVerifiedCount = annotation.dafnyVerified() >= 0 ? annotation.dafnyVerified() : null;
         Integer expectedDafnyErrorCount = annotation.dafnyErrors() >= 0 ? annotation.dafnyErrors() : null;
         Assertions.assertAll(
-                () -> assertThat("exit code",
-                        verificationResults.getExitCode(),
-                        is(annotation.exitCode())),
 //                () -> assertThat("Dafny verified count",
 //                        verificationResults.getDafnyVerifiedCount(),
 //                        is(expectedDafnyVerifiedCount)),
