verifier/src/main/java/com/aws/jverify/verifier/compiler/ExpressionCompiler.java
@@ -1,11 +1,9 @@
 package com.aws.jverify.verifier.compiler;
 
-import com.aws.jverify.ContractException;
 import com.aws.jverify.Modifiable;
 import com.aws.jverify.generated.*;
 import com.aws.jverify.verifier.compiler.simplifications.JVerifyGhostExpressionCompiler;
 import com.aws.jverify.verifier.compiler.simplifications.ImmutableTypeCompiler;
-import com.sun.jdi.event.ThreadStartEvent;
 import com.sun.source.tree.Tree;
 import com.sun.tools.javac.code.Symbol;
 import com.sun.tools.javac.code.Symtab;
@@ -20,7 +18,6 @@ import javax.lang.model.type.TypeKind;
 import java.util.List;
 import java.util.Map;
 import java.util.Objects;
-import java.util.Set;
 import java.util.function.BiFunction;
 import java.util.function.Supplier;
 import java.util.stream.Stream;
@@ -355,7 +352,6 @@ public class ExpressionCompiler {
         }
 
         var methodSymbol = TreeInfo.symbol(invocation.getMethodSelect());
-        var argBindings = invocation.getArguments().stream().map(a -> new ActualBinding(null, toExpr(a), false)).toList();
 
         if (!((invocation.getMethodSelect() instanceof JCTree.JCFieldAccess fieldAccess) ||
              (invocation.getMethodSelect() instanceof JCTree.JCIdent))) {
@@ -383,10 +379,9 @@ public class ExpressionCompiler {
                 return new ExprDotName(origin, receiver, fieldName, null);
             }
         }
-        
+
         var target = toExpr(invocation.getMethodSelect());
-        return new ApplySuffix(origin, target, null,
-                new ActualBindings(argBindings), null);
+        return createCall(origin, target, invocation.getArguments().stream());
     }
 
     /**
@@ -409,9 +404,7 @@ public class ExpressionCompiler {
 
         if (opName.equals("+") && leftType.toString().contentEquals(String.class.getName())) {
             var callee = new ExprDotName(origin, left, new Name(origin, "concat"), null);
-            var arg = List.of(new ActualBinding(null, right, false));
-            return new ApplySuffix(origin, callee, null,
-                    new ActualBindings(arg), null);
+            return createCall2(origin, callee, Stream.of(right));
         }
 
         if (opName.equals("==") || opName.equals("!=")) {
@@ -526,14 +519,15 @@ public class ExpressionCompiler {
                 // Fallback to sequence of numeric values
                 var charExprs = stringValue.chars().boxed()
                         .map(c -> (Expression) new LiteralExpr(origin, c)).toList();
-                return new ApplySuffix(origin, new NameSegment(origin, "String", null), null,
-                        new ActualBindings(List.of(new ActualBinding(null, new SeqDisplayExpr(origin, charExprs), false))), null);
+                NameSegment callee = new NameSegment(origin, "String", null);
+                SeqDisplayExpr actual = new SeqDisplayExpr(origin, charExprs);
+                return createCall2(origin, callee, Stream.of(actual));
             }
         }
 
         var stringExpr = new StringLiteralExpr(origin, translatedChars.toString(), false);
-        return new ApplySuffix(origin, new NameSegment(origin, "JString", null), null,
-                new ActualBindings(List.of(new ActualBinding(null, stringExpr, false))), null);
+        NameSegment callee = new NameSegment(origin, "JString", null);
+        return createCall2(origin, callee, Stream.of(stringExpr));
     }
 
     private static final Map<Character, String> ESCAPED_CHARS = Map.of(
@@ -545,4 +539,19 @@ public class ExpressionCompiler {
             '\r', "\\r",
             '\t', "\\t"
     );
+
+
+    public ApplySuffix createCall(IOrigin origin, Expression callee, Stream<JCTree.JCExpression> arguments) {
+        return createCall2(origin, callee, arguments.map(this::toExpr));
+    }
+
+    public static ApplySuffix createCall2(IOrigin origin, Expression callee, Stream<Expression> bindingList) {
+        return new ApplySuffix(origin, callee, null,
+                createBindings(bindingList), null);
+    }
+
+    public static ActualBindings createBindings(Stream<Expression> bindingList) {
+        return new ActualBindings(bindingList.map(expression ->
+                new ActualBinding(null, expression, false)).toList());
+    }
 }
